FSharpNemlogIn/FStarWrapper/Program.fs
@@ -5,9 +5,14 @@ open CryptoTest
 
 [<EntryPoint>]
 let main argv = 
-    let _ = TestCrypto  
-        
-    //    let _ = X.CreateSendAndRecieve "sp" "idp"
+    
+//    let keys = Protocol.KeyGenExt "me"
+//    let priv = keys.__tag
+    
+    //let _ = TestCrypto  
+    let req = X.GetSamlMessages "sp" "idp"
+            
+    let _ = X.CreateSendAndRecieve "sp" "idp"
    
     let key = Console.Read ()
     0 // return an integer exit code
