Protocol/ServiceProvider.fst
@@ -4,27 +4,23 @@ open Protocol
 val serviceprovider:  me:prin -> pubkey me -> privkey me ->
                       browser:prin -> idp:prin -> pubkey idp -> unit 
 let serviceprovider me pubk privk browser idp pubkidp = 
-  let reqRes = Recieve browser in (*1*)
+  let reqRes = Recieve browser in (*1*) (*7*)
   match reqRes with
   | HttpGet (uri) -> 
-  
+
     let authnReq = CreateAuthnRequest me idp in 
     assume(Log me authnReq) (*Protocol event*);
     let sigSP = Sign me privk authnReq in
       
     let authnReqest = SamlProtocolMessage idp authnReq sigSP in 
-    Send browser authnReqest; (*2*)  
-    let authResponse = Recieve browser in (*7*)
-    match authResponse with
-    | SamlProtocolMessage (sp, msg, sigIDP) -> 
-      (if VerifySignature idp pubkidp msg sigIDP
+    Send browser authnReqest (*2*)  
+
+  | SamlProtocolMessage (sp, msg, sigIDP) -> 
+      if VerifySignature idp pubkidp msg sigIDP
       then
         (assert(Log idp msg);
-          let resource = Resource uri in
+          let resource = Resource "uri" in
           Send browser resource)  (*8*)
-      else ())
-    | _ ->  Send browser (Failed (403))(*8.1*)     
+      else Send browser (Failed (403))(*8.1*)
   
   | _ -> Send browser (Failed (400))(*2.1*)
-
-end (* Serviceprovider *)
